\documentclass{report}

\usepackage[utf8]{inputenc}
\usepackage{amsmath}
\usepackage{amsfonts}
\usepackage{amsthm}
\usepackage{enumerate}

\theoremstyle{definition}
\newtheorem{exerciseimpl}{Exercise}
\newenvironment{exercise}[1]{
  \renewcommand\theexerciseimpl{#1}
  \exerciseimpl
}{\endexerciseimpl}

\newcommand{\slfrac}[2]{\left.#1\middle/#2\right.}
\DeclareMathOperator{\E}{\mathbb{E}}
\renewcommand{\P}[1]{\mathbb{P}\left\{#1\right\}}
\newcommand{\ind}[1]{\mathbf{1}_{\left\{#1\right\}}}
\DeclareMathOperator{\Var}{\mathrm{Var}}

\title{Notes on High-Dimensional Probability \linebreak[1] by Roman Vershynin}
\author{Tavian Barnes}
\date{}


\begin{document}

\maketitle

\chapter*{Appetizer: Using Probability to Cover a Geometric Set}

\begin{exercise}{0.0.3}~
  \begin{enumerate}[(a)]
  \item
    \begin{align*}
      \E \left\| \sum_{j=1}^k Z_j \right\|_2^2 & = \E \sum_{i=1}^n \left(\sum_{j=1}^k Z_{j,i}\right)^2 \\
      & = \E \sum_{i=1}^n \sum_{j=1}^k \sum_{m=1}^k Z_{j,i} Z_{m,i} \\
      & = \E \sum_{i=1}^n \left(\sum_{j=1}^k Z_{j,i}^2 + \sum_{j=1}^k \sum_{\substack{m=1 \\ m \ne j}}^k Z_{j,i} Z_{m,i}\right) \\
      & = \sum_{j=1}^k \E \sum_{i=1}^n Z_{j,i}^2 + \sum_{i=1}^n \sum_{j=1}^k \sum_{\substack{m=1 \\ m \ne j}}^k \E (Z_{j,i} Z_{m,i}) \\
      & = \sum_{j=1}^k \E \|Z_j\|_2^2 + \sum_{i=1}^n \sum_{j=1}^k \sum_{\substack{m=1 \\ m \ne j}}^k (\E Z_{j,i}) (\E Z_{m,i}) \tag{by independence} \\
      & = \sum_{j=1}^k \E \|Z_j\|_2^2.
    \end{align*}

  \item
    \begin{align*}
      \E \|Z - \E{Z}\|_2^2 & = \E \sum_{i=1}^n (Z_i - \E{Z_i})^2 \\
      & = \E \sum_{i=1}^n (Z_i^2 - 2 Z_i \E{Z_i} + (\E{Z_i})^2) \\
      & = \E \sum_{i=1}^n Z_i^2 - 2 \sum_{i=1}^n \E Z_i \E{Z_i} + \sum_{i=1}^n (\E Z_i)^2 \\
      & = \E \sum_{i=1}^n Z_i^2 -  \sum_{i=1}^n (\E Z_i)^2 \\
      & = \E \|Z\|_2^2 - \|\E Z\|_2^2
    \end{align*}
  \end{enumerate}
\end{exercise}

\begin{exercise}{0.0.5}
  The first inequality:
  \begin{align*}
    \left(\frac{n}{m}\right)^m & = \frac{n}{m} \left(\frac{n}{m}\right)^{m-1} \\
    & \le \frac{n}{m} \left(\frac{n-1}{m-1}\right)^{m-1} \\
    & \le \frac{n}{m} \frac{n-1}{m-1} \cdots \frac{n-m+1}{1} \\
    & = \binom{n}{m}. \\
    \intertext{The second:}
    \binom{n}{m} & \le \binom{n}{m} + \sum_{k=0}^{m-1} \binom{n}{k} \\
    & = \sum_{k=0}^m \binom{n}{k}. \\
    \intertext{The third:}
    \sum_{k=0}^m \binom{n}{k} \left(\frac{m}{n}\right)^m & \le \sum_{k=0}^m \binom{n}{k} \left(\frac{m}{n}\right)^k \\
    & = \left(1 + \frac{m}{n}\right)^m, \\
    \intertext{therefore}
    \sum_{k=0}^m \binom{n}{k} & \le \left(1 + \frac{m}{n}\right)^m \left(\frac{n}{m}\right)^m. \\
    & = \left(\frac{n + m}{m}\right)^m \\
    & \le \left(\frac{e n}{m}\right)^m.
  \end{align*}
\end{exercise}

\begin{exercise}{0.0.6}
\end{exercise}


\chapter{Preliminaries on Random Variables}

\begin{exercise}{1.2.2}
  Split $X$ into its positive and negative part, and apply Lemma 1.2.1 to each:
  \begin{align*}
    \E X & = \E (X \ind{X \ge 0} - (-X \ind{X < 0})) \\
    & = \int_0^\infty \P{X \ind{X \ge 0} > t} dt - \int_{0}^{\infty} \P{-X \ind{X < 0} > t} dt \\
    & = \int_0^\infty \P{X > t} dt - \int_{-\infty}^0 \P{X < t}
  \end{align*}
\end{exercise}

\begin{exercise}{1.2.3}
  By Lemma 1.2.1,
  \begin{align*}
    \E |X|^p & = \int_0^\infty \P{|X|^p > u} du. \\
    \intertext{Making the substitution $u = t^p$, $du = p t^{p-1} dt$, this equals}
    & \mathrel{\phantom{=}} \int_0^\infty p t^{p-1} \P{|X|^p > t^p} dt \\
    & = \int_0^\infty p t^{p-1} \P{|X| > t} dt.
  \end{align*}
\end{exercise}

\begin{exercise}{1.2.6}
  \begin{align*}
    \P{|X - \mu| \ge t} & = \P{(X - \mu)^2 \ge t^2} \\
    & \le \frac{\E (X - \mu)^2}{t^2} \\
    & = \frac{\sigma^2}{t^2}.
  \end{align*}
\end{exercise}

\begin{exercise}{1.3.3}
  Let $\sigma^2 = \Var(X_i)$.
  \begin{align*}
    \left(\E \left|\frac{1}{N} \sum_{i=1}^N X_i - \mu\right|\right)^2 & \le \E \left(\frac{1}{N} \sum_{i=1}^N X_i - \mu\right)^2 \tag{by Jensen's inequality} \\
    & = \Var \left(\frac{1}{N} \sum_{i=1}^N X_i\right) \\
    & = \frac{\sigma^2}{N}. \tag{by equation 1.5}
  \end{align*}
\end{exercise}

\end{document}
